proofs/AdmissibilityGraph/README.md
@@ -1,3 +1,311 @@
 # Admissibility graphs
 
-This directory presents an original notion we call the *admissibility graph*.
+The theory of *admissibility graphs* is a general mathematical framework for precisely and concisely specifying encapsulation boundaries in a system. I developed this theory for a particular project, but I think it's interesting and general enough to share. This directory contains a formalization of the concept and mechanized proofs of some basic theorems about it. This document is an informal introduction to the idea.
+
+## Motivation
+
+Imagine a simple sorting program that reads in some lines of text and prints them out in lexicographical order. A simplified [static call graph](https://en.wikipedia.org/wiki/Call_graph) for that program might look as follows:
+
+```mermaid
+flowchart TD
+  main([main])
+  quicksort([quicksort])
+  partition([partition])
+  read([read_line])
+  print([print_line])
+
+  main --> quicksort
+  quicksort --> partition
+  quicksort --> quicksort
+  main --> read
+  main --> print
+```
+
+For encapsulation purposes, you may wish to decree that `partition` is an implementation detail of `quicksort` and should not be called from any other function. Equivalently, you'd like to forbid any edges to `partition` in the call graph except the one from `quicksort`. How should a programmer express that?
+
+Of course, most programming languages already have a mechanism for information hiding—or several! For example, [scoping](https://en.wikipedia.org/wiki/Scope_\(computer_science\)) allows a programmer to write local definitions which are only accessible to part of the program. Object-oriented programmers may also think of [access modifiers](https://docs.oracle.com/javase/tutorial/java/javaOO/accesscontrol.html) like `public`, `private`, and `protected`, or the concept of "[friend classes](https://en.cppreference.com/w/cpp/language/friend)" in C++. Functional programmers may be reminded of [module systems](https://jozefg.bitbucket.io/posts/2015-01-08-modules.html) or [existential quantification](https://groups.seas.harvard.edu/courses/cs152/2014sp/lectures/lec17-existential.pdf). The theory of admissibility graphs suggests a new way of understanding such language features by identifying what information the programmer should provide in order to specify encapsulation boundaries.
+
+One might wonder why any innovation is needed at all. For the call graph example, it's easy to imagine an "access graph" with the same nodes, using edges in the access graph to indicate which edges should be allowed in the call graph. Then an edge in the call graph implies a corresponding edge in the access graph. Stated differently, the lack of an edge in the access graph demands the lack of an edge in the call graph. Unfortunately, this isn't very useful, since an access graph like that would be too large for a programmer to comfortably manage. For example, suppose some component of the program consists of 10 functions which should all be able to call each other. Then the access subgraph for those functions would have 10² = 100 edges, and introducing a new function would require adding 11² - 10² = 21 new access edges! The programmer shouldn't have to specify this much data to encode an intention as mundane as "unrestricted mutual access".
+
+Our thesis is that the programmer should instead specify their access policies in the form of an admissibility graph, which will be defined below.
+
+As abstract mathematical objects, admissibility graphs are not specifically about computer programs. For example, a cloud computing provider might consider using admissibility graphs as a form of [IAM](https://docs.aws.amazon.com/IAM/latest/UserGuide/access_policies.html) configuration. However, we'll stick to the theme of encapsulation in computer programs for our examples.
+
+## The definition
+
+Before we look at any particular admissibility graphs, allow me to first define the abstract concept.
+
+### The data
+
+An admissibility graph, like any graph, has a set of *nodes*. The nodes might represent entities such as functions or modules in a program.
+
+An admissibility graph has two types of directed edges between nodes:
+
+- **References** are the main edges of the graph. They might represent associations like function calls or module imports in a program. A reference is represented as a solid arrow from a *source* node to a *target* node.
+
+  ```mermaid
+  ---
+  title: Reference
+  ---
+  flowchart LR
+    source([source])
+    target([target])
+
+    source --> target
+  ```
+
+- **Parent-child relationships**, as we'll soon see, organize the nodes in a way that restricts which references are allowed to exist. A parent-child relationship is represented as a dotted arrow from a *parent* node to a *child* node.
+
+  ```mermaid
+  ---
+  title: Parent-child relationship
+  ---
+  flowchart LR
+    parent([parent])
+    child([child])
+
+    parent -.-> child
+  ```
+
+These two types of edges are understood as binary relations on nodes, since there is no need to consider multiple edges of the same type between two nodes.
+
+### The axioms
+
+We impose a couple of requirements on admissibility graphs. Before we get to them, we must define the following:
+
+- *Ancestry* is the [reflexive](https://en.wikipedia.org/wiki/Reflexive_closure) [transitive closure](https://en.wikipedia.org/wiki/Transitive_closure) of the parent-child relation. In other words, `A` is an ancestor of `D` (`D` is a descendant of `A`) when there is a (possibly empty) path from `A` to `D` consisting of parent-child relationships. In English, "ancestry" is not typically thought of as being a reflexive relation, but for technical reasons we define it as such.
+- A hypothetical reference from a source `S` to a target `T` is *admissible* when there exists an ancestor `A` of `S` and a descendant `D` of `T` such that `A` is a parent of `D` (`D` is a child of `A`).
+
+Now, the axioms:
+
+- **Antisymmetry:** If two nodes are ancestors of each other, then they're the same node.
+- **Admissibility:** Every reference is admissible.
+
+The [antisymmetry](https://en.wikipedia.org/wiki/Antisymmetric_relation) axiom simplifies reasoning about the graph without any loss of generality. It implies that the parent-child relation is a [partial order](https://en.wikipedia.org/wiki/Partially_ordered_set), or equivalently that the parent-child relationships induce a [directed acyclic subgraph](https://en.wikipedia.org/wiki/Directed_acyclic_graph). Note that antisymmetry only applies to ancestry (and thus parent-child relationships), not to references.
+
+The admissibility axiom enforces encapsulation boundaries in the graph. The definition of admissible might seem obtuse, but we'll come to understand it through examples below.
+
+## Examples
+
+### Trivial admissibility graphs
+
+The simplest possible admissibility graph has no nodes, and thus no references or parent-child relationships. It's not very interesting. We can also consider an admissibility graph with one node and no references or parent-child relationships, but it's not very interesting either.
+
+```mermaid
+---
+title: Valid
+---
+flowchart TD
+  a([A])
+```
+
+### Self-references
+
+The following is not a valid admissibility graph:
+
+```mermaid
+---
+title: Invalid
+---
+flowchart TD
+  a([A])
+
+  a --> a
+```
+
+The problem is that `A` references itself, but the reference is not admissible. In other words, we have not given `A` permission to access itself. We can fix that by making `A` a parent of itself.
+
+```mermaid
+---
+title: Valid
+---
+flowchart TD
+  a([A])
+
+  a -.-> a
+  a --> a
+```
+
+### Parents and children
+
+The following is not a valid admissibility graph:
+
+```mermaid
+---
+title: Invalid
+---
+flowchart LR
+  a([A])
+  b([B])
+
+  a --> b
+```
+
+The problem is that `A` references `B`, but the reference is not admissible. We can fix that in two ways by making either node a parent of the other.
+
+```mermaid
+---
+title: Valid
+---
+flowchart TD
+  a([A])
+  b([B])
+
+  a -.-> b
+  a --> b
+```
+
+```mermaid
+---
+title: Valid
+---
+flowchart TD
+  a([A])
+  b([B])
+
+  b -.-> a
+  a --> b
+```
+
+From this example, we can see that parents can access their children, and children can access their parents.
+
+### Ancestral cycles
+
+In the previous example, we encountered a problem that could be fixed by adding a parent-child relationship between two nodes in either direction. But we better not make `A` and `B` parents of each other, since that would violate antisymmetry.
+
+```mermaid
+---
+title: Invalid
+---
+flowchart TD
+  a([A])
+  b([B])
+
+  a -.-> b
+  b -.-> a
+```
+
+Any longer cycles in parent-child relationships are also forbidden by antisymmetry:
+
+```mermaid
+---
+title: Invalid
+---
+flowchart TD
+  a([A])
+  b([B])
+  c([C])
+
+  a -.-> b
+  b -.-> c
+  c -.-> a
+```
+
+### Grandparents and grandchildren
+
+What about grandparents?
+
+```mermaid
+---
+title: Valid
+---
+flowchart TD
+  a([A])
+  b([B])
+  c([C])
+
+  a -.-> b
+  b -.-> c
+  c --> a
+```
+
+Grandchildren are allowed to access grantparents. However, the converse is not true in general. Where did this asymmetry come from?
+
+### Siblings
+
+Consider this arrangement of a parent with two children:
+
+```mermaid
+---
+title: Valid
+---
+flowchart TD
+  a([A])
+  b([B])
+  c([C])
+
+  a -.-> b
+  a -.-> c
+  b --> c
+  c --> b
+```
+
+From this example, we can see that siblings can access each other.
+
+### Niblings
+
+The following is not a valid admissibility graph:
+
+```mermaid
+---
+title: Invalid
+---
+flowchart TD
+  a([A])
+  b([B])
+  c([C])
+  d([D])
+
+  a -.-> b
+  a -.-> c
+  c -.-> d
+  b --> d
+```
+
+The reference from `B` to `D` is not admissible.
+
+From this example, we can see that nodes don't have automatic access to their [niblings](https://www.merriam-webster.com/words-at-play/words-were-watching-nibling) (children of siblings), since they are considered implementation details of their parents.
+
+### Piblings
+
+Consider the following admissibility graph:
+
+```mermaid
+---
+title: Valid
+---
+flowchart TD
+  a([A])
+  b([B])
+  c([C])
+  d([D])
+
+  a -.-> b
+  a -.-> c
+  c -.-> d
+  d --> b
+```
+
+From this example, we can see that nodes can access their [piblings](https://www.dictionary.com/e/aunt-uncle-niece-nephew-words/) (siblings of parents).
+
+Furthermore, the following is accepted:
+
+```mermaid
+---
+title: Valid
+---
+flowchart TD
+  a([A])
+  b([B])
+  c([C])
+  d([D])
+  e([E])
+
+  a -.-> b
+  b -.-> c
+  c -.-> d
+  a -.-> e
+  d --> e
+```
+
+So nodes can access the siblings of any of their ancestors, not just those of their parents.
